move things around so it compiles and runs

dafny/top-down/top-down.dfy
@@ -30,9 +30,10 @@ search(goal: SearchClause) returns (ghost proof: Option<ProofTree>, b: bool)
 */
 
 method find_matching_rules(rules: seq<Rule>, goal:SearchClause) returns (c:seq<Rule>)
+    requires valid_program(rules)
     ensures forall r:Rule :: r in c ==> r.head.name == goal.name && |r.head.terms| == |goal.evar_terms|
-    ensures forall r:Rule :: r in c ==> r.head == goal.clause
-    ensures forall r:Rule :: r in c ==> r in rules
+    // ensures forall r:Rule :: r in c ==> r.head == goal.clause
+    ensures forall r:Rule :: r in c ==> r in rules && valid_rule(r)
 {
     var matching_rules : seq<Rule> := [];
     
@@ -49,41 +50,82 @@ method find_matching_rules(rules: seq<Rule>, goal:SearchClause) returns (c:seq<R
     return matching_rules;
 }
 
+/*
+Goal = A(evar1, evar1) (A(Y,Y)) goal.subst == Y-->evar1
+RuleHead = A("x", X)
+
+resolve evar1 to "x"
+subst == X-->evar1
+-----------------------------
+Goal = A(evar1, evar2) (A(X, Y)) goal.subst == X-->evar1, Y-->evar2
+RuleHead = A(P, P)
+
+in unify of A(P, P)
+    if P in subst already:
+        update goal.subst such that everything that mapped to evar2 now maps to subst[P]
+subst == P-->evar1, P-->evar2
+
+*/
 
 method unify(head_clause:Clause, goal:SearchClause, emap:EvarMap) returns (o:Option<EvarSubstitution>)//, e:EvarMap)
     requires emap.inv()
+    requires valid_clause(head_clause)
     requires |head_clause.terms| == |goal.evar_terms|
     requires goal.valid()
     requires goal.valid_emap(emap)
+    requires goal.name == head_clause.name
     modifies emap
     ensures emap.is_more_resolved()
     ensures goal.valid_emap(emap)
     ensures emap.inv()
-    ensures o.Some? ==> forall e :: e in o.value.Values ==> e in emap.evar_map
-    ensures o.Some? ==> forall v :: v in goal.clause.terms && v.Var? ==> v in o.value
-    ensures head_clause.is_ground() && o.Some? ==> goal.emap_fully_resolved(emap)
+    ensures o.Some? ==> o.value.valid()
+    // ensures o.Some? ==> forall e :: e in o.value.Values ==> e in emap.evar_map
+    ensures o.Some? ==> forall e :: o.value.in2(e) ==> e in emap.evar_map
+    // ensures o.Some? ==> forall v :: v in goal.clause.terms && v.Var? ==> o.value.in1(v) // IS WRONG
+    ensures o.Some? ==> forall v :: v in head_clause.terms ==> o.value.in1(v)
+    ensures head_clause.is_ground() && o.Some? ==> goal.emap_fully_resolved(emap) // o.value is empty map
+    ensures head_clause.is_ground() && o.Some? ==> goal.clause.make_fact(make_subst(emap, goal.subst)) == head_clause
+    // ensures o.Some? ==> goal.clause.make_fact(make_subst(emap,goal.subst)) == head_clause.make_fact(make_subst(emap,o.value))
     ensures emap.monotonically_increasing() // ensures forall e :: e in old(emap.evar_map) ==> e in emap.evar_map
+    ensures o.Some? ==> forall i:nat | i < |head_clause.terms| :: o.value.get1(head_clause.terms[i]) == goal.evar_terms[i]
+    // ensures forall v :: goal.subst.in1(v) && v.Var? && o.Some? ==> o.value.in1(v) && goal.subst.get1(v) == o.value.get1(v)
+    // ensures o.Some? ==> forall i:nat | i < |head_clause.terms| ::
+    //                       (if head_clause.terms[i].Var? then o.value.get1(head_clause.terms[i]) == goal.evar_terms[i]
+    //                       else emap.evar_map[goal.evar_terms[i]].Some?)
+    ensures o.Some? ==> forall j :: 0 <= j < |head_clause.terms| ==> head_clause.terms[j].Const? ==> emap.evar_map[goal.evar_terms[j]].Some? && Const(emap.evar_map[goal.evar_terms[j]].value) == head_clause.terms[j]
+    // |goal.evar_terms| == |o.value.Values| // is this true?
+    
 {
     // check if all terms in clause have correct mapping in goal.evar_terms
-    var subst:EvarSubstitution := map[];
-    for i := 0 to |head_clause.terms| 
+    var subst:EvarSubstitution := new_bijective_map<VarTerm, Evar>();
+    for i := 0 to |head_clause.terms|
         invariant emap.inv()
+        invariant subst.valid()
+        invariant goal.valid()
         invariant goal.valid_emap(emap)
-        invariant forall e :: e in subst.Values ==> e in emap.evar_map
+        invariant forall e :: subst.in2(e) ==> e in emap.evar_map
         invariant emap.monotonically_increasing() // invariant forall e :: e in old(emap.evar_map) ==> e in emap.evar_map
         invariant emap.is_more_resolved()
-        invariant forall j :: 0 <= j < i ==> head_clause.terms[j].Const? ==> emap.evar_map[goal.evar_terms[j]].Some?
+        invariant forall j :: 0 <= j < i ==> subst.in1(head_clause.terms[j]) && subst.get1(head_clause.terms[j]) == goal.evar_terms[j]
+        // invariant forall j:nat | j < i && head_clause.terms[j].Var? :: subst.get1(head_clause.terms[j]) == goal.evar_terms[j]
+        invariant forall j :: 0 <= j < i ==> head_clause.terms[j].Const? ==> emap.evar_map[goal.evar_terms[j]].Some? && Const(emap.evar_map[goal.evar_terms[j]].value) == head_clause.terms[j]
+        invariant forall j :: i <= j < |head_clause.terms| ==> !subst.in1(head_clause.terms[j])
+        invariant forall j :: i <= j < |goal.evar_terms| ==> !subst.in2(goal.evar_terms[j])
+        // invariant forall j:nat | j < i :: goal.subst.in1(goal.clause.terms[i]) && goal.clause.terms[i].Var? ==> subst.in1(goal.clause.terms[i]) && goal.subst.get1(goal.clause.terms[i]) == subst.get1(head_clause.terms[i])
+        // invariant head_clause.is_ground() ==> forall j:nat :: j < i ==> goal.clause.make_fact(make_subst(emap, goal.subst)).terms[j] == head_clause.terms[j]
     {
         if head_clause.terms[i].Var? {
             //print "a";
             var variableName := head_clause.terms[i].s;
-            subst := subst[head_clause.terms[i] := goal.evar_terms[i]];
+            // subst := subst[head_clause.terms[i] := goal.evar_terms[i]];
+            subst := subst.insert(head_clause.terms[i], goal.evar_terms[i]);
         } else if head_clause.terms[i].Const? {
             //print "b";
             var constant := head_clause.terms[i].c;
             var e := emap.lookup(goal.evar_terms[i]);
             match e {
                 case None => {
+                    subst := subst.insert(head_clause.terms[i], goal.evar_terms[i]);
                     emap.resolve(goal.evar_terms[i], constant);
                 }
                 case Some(constant') =>
@@ -91,119 +133,144 @@ method unify(head_clause:Clause, goal:SearchClause, emap:EvarMap) returns (o:Opt
                         // ignore rule
                         return None;
                     }
-                    // } else {
-                    //     subst := subst[head_clause.terms[i] := goal.evar_terms[i]];
-                    // }
+                    else {
+                        subst := subst.insert(head_clause.terms[i], goal.evar_terms[i]);
+                    }
             }
         }
     }
     reveal ToSet();
+    // assert(head_clause.is_ground() ==> forall i:nat :: i < |goal.clause.terms| ==> make_subst(emap, goal.subst)[goal.clause.terms[i]].c == emap.evar_map[goal.evar_terms[i]].value);
+    // assert(head_clause.is_ground() ==> forall i:nat :: i < |goal.clause.terms| ==> make_subst(emap, goal.subst)[goal.clause.terms[i]] == goal.clause.make_fact(make_subst(emap, goal.subst)).terms[i]);
+    // assert(head_clause.is_ground() ==> forall i:nat :: i < |goal.clause.terms| ==> goal.clause.make_fact(make_subst(emap, goal.subst)).terms[i] == head_clause.terms[i]);
     return Some(subst);
 }
 
 method evarify(clause:Clause, subst:EvarSubstitution, emap:EvarMap) 
     returns (sc:SearchClause, subst':EvarSubstitution)
     requires emap.inv()
-    requires forall e :: e in subst.Values ==> e in emap.evar_map
+    requires subst.valid()
+    requires valid_clause(clause)
+    requires forall e :: subst.in2(e) ==> e in emap.evar_map
     modifies emap
+    ensures  subst'.valid()
     ensures  emap.inv()
+    ensures  sc.subst.valid()
+    ensures  sc.valid()
     ensures  sc.valid_emap(emap)
-    ensures  forall e :: e in subst'.Values ==> e in emap.evar_map
+    ensures  forall e :: subst'.in2(e) ==> e in emap.evar_map
+    ensures  forall e :: sc.subst.in2(e) ==> e in emap.evar_map
     ensures  emap.monotonically_increasing() // ensures forall e :: e in old(emap.evar_map) ==> e in emap.evar_map
-    ensures  forall s :: s in subst ==> s in subst'
+    ensures  forall s :: subst.in1(s) ==> subst'.in1(s) && subst.get1(s) == subst'.get1(s)
     ensures  sc.clause == clause
     ensures  sc.clause.substitution_complete(make_subst(emap, subst'))
-    ensures  sc.valid()
+    // ensures  sc.subst.IsSubsetOf(subst') // sc.subst.Items() <= subst'.Items()
+    ensures  forall v :: sc.subst.in1(v) && v.Var? ==> subst'.in1(v) && sc.subst.get1(v) == subst'.get1(v)
+    // ensures forall e :: e in subst'
 {
     subst' := subst;
-    var local_subst:EvarSubstitution := map[];
+    var local_subst:EvarSubstitution := new_bijective_map<VarTerm, Evar>();
     var evar_terms:seq<Evar> := [];
     reveal ToSet();
     for i := 0 to |clause.terms|
         invariant emap.inv()
+        invariant subst'.valid()
+        invariant local_subst.valid()
+        // invariant forall j :: j < i ==> 
         invariant forall e :: e in evar_terms ==> e in emap.evar_map
-        invariant forall e :: e in subst'.Values ==> e in emap.evar_map
+        invariant forall e :: subst'.in2(e) ==> e in emap.evar_map
         invariant emap.monotonically_increasing() // invariant forall e :: e in old(emap.evar_map) ==> e in emap.evar_map 
-        invariant forall s :: s in subst ==> s in subst'
-        invariant forall j :: 0 <= j < i ==> clause.terms[j].Var? ==> clause.terms[j] in subst'
-        invariant forall e :: e in local_subst.Values ==> e in evar_terms
+        invariant  forall s :: subst.in1(s) ==> subst'.in1(s) && subst.get1(s) == subst'.get1(s)
+        invariant forall j :: 0 <= j < i ==> clause.terms[j].Var? ==> subst'.in1(clause.terms[j])
+        invariant forall e :: local_subst.in2(e) ==> e in evar_terms
+        // invariant local_subst.Keys() <= subst'.Keys()
+        // invariant local_subst.Items() <= subst'.Items()
+        // invariant local_subst.Values() <= subst'.Values()
+        invariant forall j :: i <= j < |clause.terms| ==> !local_subst.in1(clause.terms[j])
+        invariant forall j :: i <= j < |clause.terms| ==> (subst'.in1(clause.terms[j])) ==> !local_subst.in2(subst'.get1(clause.terms[j]))
+        invariant |evar_terms| == i
+        invariant reveal ToSet(); local_subst.Values() == ToSet(evar_terms)
+        invariant forall j:nat | j < i :: local_subst.in1(clause.terms[j]) && (local_subst.get1(clause.terms[j]) == evar_terms[j])
+        invariant forall v :: local_subst.in1(v) && v.Var? ==> subst'.in1(v) && local_subst.get1(v) == subst'.get1(v)
+        invariant forall j:nat | 0 <= j < i :: clause.terms[j].Const? ==> emap.evar_map[evar_terms[j]] == Some(clause.terms[j].c)
+        // invariant forall e :: e in local_subst.l_to_r ==> e in subst'.l_to_r
     {
         var term := clause.terms[i];
         match term {
             case Var(s) => {
-                if term in subst'.Keys {
-                    var ev := subst'[term]; // this should imply ev in emap.evar_map
+                if subst'.in1(term) {
+                    var ev := subst'.get1(term); // this should imply ev in emap.evar_map
                     evar_terms := evar_terms + [ev];
-                    local_subst := local_subst[term := ev];
-                } else if term !in subst' {
+                    // local_subst := local_subst[term := ev];
+                    // assert(!local_subst.in1(term));
+                    // assert(!local_subst.in2(ev));
+                    local_subst := local_subst.insert(term , ev);
+                } else if !subst'.in1(term) { // TODO: THIS SHOULDN'T HAPPEN IF THE rule_restricted thing is there
                     var new_ev := emap.get_new_evar();
                     evar_terms := evar_terms + [new_ev];
-                    subst' := subst'[term := new_ev];
-                    local_subst := local_subst[term := new_ev];
+                    // subst' := subst'[term := new_ev];
+                    // InsertPreservesSubset(local_subst, subst', term, new_ev);
+                    subst' := subst'.insert(term, new_ev);
+                    // local_subst := local_subst[term := new_ev];
+                    local_subst := local_subst.insert(term, new_ev);
                 }
             }
             case Const(c) => {
                 var new_ev := emap.get_new_evar();
                 evar_terms := evar_terms + [new_ev];
                 emap.resolve(new_ev, c);
+                local_subst := local_subst.insert(term, new_ev);
             }
         }
     }
-
+    assert(|evar_terms| == |clause.terms|);
     sc := SearchClause(clause.name, evar_terms, clause, local_subst);
 }
+
+/*
+forall sc:SearchClause, forall emap:EvarMap, if sc.emap_fully_resolved(old(emap)) && emap.monotonically_increasing() then sc.emap_fully_resolved(emap)
+*/
 
 method search (rules:seq<Rule>, goal:SearchClause, emap:EvarMap, depth: nat) returns (b:bool, ghost proof: Option<Proof>)//, e:EvarMap)
     requires valid_program(rules)
     requires emap.inv()
-    requires goal.valid_emap(emap)
     requires goal.valid()
+    requires goal.valid_emap(emap)
     // ensures o.Some? ==> forall e :: e in o.value.Values ==> e in emap.evar_map
     modifies emap
     ensures emap.inv()
     ensures goal.valid_emap(emap) // TODO: Do we need to prove this at all times?
     ensures emap.monotonically_increasing() // ensures forall e :: e in old(emap.evar_map) ==> e in emap.evar_map
-    ensures b ==> proof.Some? && valid_proof(rules, goal.clause, proof.value)
-    ensures b ==> goal.emap_fully_resolved(emap)
+    // ensures b ==> goal.emap_fully_resolved(emap)
+    ensures b ==> goal.clause.substitution_concrete(make_subst(emap, goal.subst))
+    ensures b ==> proof.Some? && valid_proof(rules, goal.clause.make_fact(make_subst(emap, goal.subst)), proof.value)
+    // ensures b ==> proof.Some? && Last(proof.value).new_fact() == goal.clause.make_fact(make_subst(emap, goal.subst))
+    // ensures emap.is_more_resolved'()
     decreases depth
-    // what the correct matching rule is (rule for which we returned true)
-    //   - maybe return a sequence of these rules
-    //   - build a 'substitution' map like Bryan using these rules
-    //       - a substitution is either a variable->evar or evar->const(resolve)
-    //   - ??
-    //   - reuse Bryan's spec
-    // ensures b ==> that rule works
-
-    // the different subst bi-maps are consistent // WRONG
-    // we should somehow say b==true ==> at no point we made the same evar resolve to two diff consts
-    // for each subst (at each instantiation of a rule down the tree), convert that subst into Bryan's substitution (using the 'global' evarmap)
-    //  -- keep a ghost state of seq<subst * rule> or a seq<applied_rules> * seq<subst for that rule>?
-    //  -- (var -> evar -> const) ==> (var -> const) like Bryan's substitution (a ground substitution)
-    //  -- do the above for ALL evars in our evarmap, the one for which search returns true (basically for all evars we want them to be present in substs)
-    //  --   at each proofstep, the number of evars for which the above stuff is not done decreases
-    // prove completeness of our substs? - we get a valid ProofStep for free?
 {
     if (depth == 0) {
         return false, None;
     }
-    //print "Searching on ", goal, " with emap ", emap.evar_map, "\n";
+    var current_emap:EvarMap := new EvarMap.Init(emap);
     // find all rules that match current goal
     var matching_rules := find_matching_rules(rules, goal);
-    //print "\t matching_rules = ", matching_rules, "\n";
-
+    assert(forall r :: r in matching_rules ==> valid_clause(r.head) && (forall c :: c in r.body ==> valid_clause(c)));
     // for all rules that match the current goal
+    label AA: 
     for i := 0 to |matching_rules|
         invariant emap.inv()
+        invariant current_emap.inv()
+        invariant old@AA(current_emap.evar_map) == current_emap.evar_map
+        invariant old@AA(current_emap.next_evar) == current_emap.next_evar
+        // invariant unchanged@AA(current_emap)
+        invariant forall j:nat | j < i :: valid_rule(matching_rules[j])
         // invariant goal.valid_emap(emap)
         invariant emap.monotonically_increasing() // invariant forall e :: e in old(emap.evar_map) ==> e in emap.evar_map
     {
-        //print "\t i = ", i, "\n"; 
-        var current_emap:EvarMap := new EvarMap.Init(emap); // TODO: Check if this actually makes a copy
+        emap.copy(current_emap);
         var rule:Rule := matching_rules[i];
-        //print "\t matching_rule = ", rule, "\n";
+        assert(valid_clause(rule.head));
         var option_subst := unify(rule.head, goal, emap);
-        
-        //print "\t option_subst = ", option_subst, "\n";
         
         var subst : EvarSubstitution;
         match option_subst {
@@ -214,22 +281,34 @@ method search (rules:seq<Rule>, goal:SearchClause, emap:EvarMap, depth: nat) ret
         var search_clauses:seq<SearchClause> := [];
         if |rule.body| == 0 {
             var concreteSubst := make_subst(emap, subst);
-            var proofStep := ProofStep(concreteSubst, rule, []);
+            var proofStep := ProofStep(map[], rule, []);
             assert rule in rules; // needed to use valid_program(rules) to conclude that valid_rule(rule) and then conclude that rule.head.is_ground() 
+            // assume (goal.clause.make_fact(make_subst(emap, goal.subst)) == rule.head.make_fact(concreteSubst));
             return true, Some([proofStep]);
         } else {
             for j := 0 to |rule.body|
                 invariant |search_clauses| == j
                 invariant emap.inv()
                 invariant current_emap.inv()
+                // invariant unchanged@AA(current_emap)
+                invariant old@AA(current_emap.evar_map) == current_emap.evar_map
+                invariant old@AA(current_emap.next_evar) == current_emap.next_evar
+                invariant subst.valid()
                 // invariant current_emap.evar_map == old(current_emap.evar_map)
+                invariant forall sc :: sc in search_clauses ==> sc.valid()
                 invariant forall sc :: sc in search_clauses ==> sc.valid_emap(emap)
-                invariant forall e :: e in subst.Values ==> e in emap.evar_map
+                invariant forall e :: subst.in2(e) ==> e in emap.evar_map
                 invariant emap.monotonically_increasing() // invariant forall e :: e in old(emap.evar_map) ==> e in emap.evar_map
                 invariant forall e :: e in old(emap.evar_map) ==> e in current_emap.evar_map // TODO: Make this a predicate inside evar.dfy
-                invariant forall i :: 0 <= i < j ==> rule.body[i] == search_clauses[i].clause;
+                invariant forall i :: 0 <= i < j ==> rule.body[i] == search_clauses[i].clause
                 invariant forall i :: 0 <= i < j ==> search_clauses[i].clause.substitution_complete(make_subst(emap, subst))
                 invariant forall i :: 0 <= i < j ==> search_clauses[i].valid()
+                invariant valid_rule(rule)
+                // invariant forall v :: goal.subst.in1(v) && v.Var? ==> subst.in1(v) && goal.subst.get1(v) == subst.get1(v)
+                invariant forall ii :: 0 <= ii < |goal.clause.terms| ==> subst.in1(rule.head.terms[ii]) && subst.get1(rule.head.terms[ii]) == goal.subst.get1(goal.clause.terms[ii])
+                invariant forall ii :: 0 <= ii < |rule.head.terms| ==> rule.head.terms[ii].Const? ==> emap.evar_map[goal.evar_terms[ii]].Some? && Const(emap.evar_map[goal.evar_terms[ii]].value) == rule.head.terms[ii];
+                invariant forall i :: 0 <= i < j ==> forall v :: search_clauses[i].subst.in1(v) && v.Var? ==> subst.in1(v) && search_clauses[i].subst.get1(v) == subst.get1(v)
+                // invariant forall k in old(subst) ==> k in subst
             {
                 var clause:Clause := rule.body[j];
                 var search_clause, subst' := evarify(clause, subst, emap);
@@ -239,48 +318,116 @@ method search (rules:seq<Rule>, goal:SearchClause, emap:EvarMap, depth: nat) ret
             var flag := true;
             ghost var proofs : seq<Proof> := [];
             assert forall i :: 0 <= i < |search_clauses| ==> search_clauses[i].clause.substitution_complete(make_subst(emap, subst));
-            for j := 0 to |search_clauses|
+            label L: for j := 0 to |search_clauses|
                 invariant emap.inv()
                 invariant current_emap.inv()
+                // invariant unchanged@AA(current_emap)
+                invariant old@AA(current_emap.evar_map) == current_emap.evar_map
+                invariant old@AA(current_emap.next_evar) == current_emap.next_evar
+                invariant subst.valid()
+                invariant forall e :: subst.in2(e) ==> e in emap.evar_map
                 // invariant current_emap == old(current_emap)
+                invariant forall sc :: sc in search_clauses ==> sc.valid()
                 invariant forall sc :: sc in search_clauses ==> sc.valid_emap(emap)
                 // invariant forall e :: e in subst.Values ==> e in emap.evar_map
-                invariant emap.monotonically_increasing() // invariant forall e :: e in old(emap.evar_map) ==> e in emap.evar_map
-                invariant forall e :: e in old(emap.evar_map) ==> e in current_emap.evar_map // TODO: Make this a predicate inside evar.dfy
+                invariant emap.monotonically_increasing@L() // invariant forall e :: e in old(emap.evar_map) ==> e in emap.evar_map
+                // invariant emap.is_more_resolved'()
+                // invariant forall e :: e in old(emap.evar_map) ==> e in current_emap.evar_map // TODO: Make this a predicate inside evar.dfy
                 // invariant goal.valid_emap(emap)
+                // invariant flag ==> forall p :: p in proofs ==> p.Some?
                 invariant flag ==> (|proofs| == j)
-                invariant flag ==> (forall i :: 0 <= i < j ==> valid_proof(rules, search_clauses[i].clause, proofs[i]))
-                invariant flag ==> forall i :: 0 <= i < j ==> search_clauses[i].clause.make_fact(make_subst(emap, subst)) == Last(proofs[i]).new_fact();
-                invariant forall e :: e in subst.Values ==> e in emap.evar_map
+                invariant flag ==> (forall i :: 0 <= i < j ==> search_clauses[i].clause == rule.body[i])
+                invariant forall c :: c in search_clauses ==> forall e :: c.subst.in2(e) ==> e in emap.evar_map
+                invariant flag ==> (forall i :: 0 <= i < j ==> search_clauses[i].clause.substitution_concrete(make_subst(emap, search_clauses[i].subst)))
+                invariant flag ==> (forall i :: 0 <= i < j ==> valid_proof(rules, search_clauses[i].clause.make_fact(make_subst(emap, search_clauses[i].subst)), proofs[i]))
+                // invariant flag ==> (forall k :: 0 <= k < j ==> search_clauses[k].emap_fully_resolved(emap))
+                invariant flag ==> forall k :: 0 <= k < j ==> search_clauses[k].clause.make_fact(make_subst(emap, search_clauses[k].subst)) == Last(proofs[k]).new_fact();
+                invariant valid_rule(rule)
+                // invariant goal.emap_fully_resolved(emap) // not true as an invariant
             {
                 var b',proof_j := search(rules, search_clauses[j], emap, depth - 1);
                 if !b' {
                     flag := false;
                     break;
                 } else {
+                    assert(proof_j.Some?);
                     proofs := proofs + [proof_j.value];
                 }
-                // current_emap := e;
+                for k := 0 to j
+                    invariant forall kk :: 0 <= kk < k ==> search_clauses[kk].valid_emap(emap)
+                {
+                    search_clauses[k].monotonically_increasing_preserves_valid_emap@L(emap);
+                }
+                assert (forall k :: 0 <= k < j ==> search_clauses[k].emap_fully_resolved(emap));
             }
             if flag {
+                /*
+                1. Use range restriction stuff to prove that emap_fully_resolved and substitution_concrete for the goal.clause
+                2. Use the fact that apply(subst, rule.head):seq<Evar> == apply(goal.subst, goal.clause):seq<Evar>
+                */
                 var concreteSubst := make_subst(emap, subst);
-                assert |proofs| == |search_clauses| == |rule.body|;
-                assert forall i :: 0 <= i < |rule.body| ==> search_clauses[i].valid_emap(emap);
-                assume forall i :: 0 <= i < |rule.body| ==> search_clauses[i].emap_fully_resolved(emap); // TODO This will depend on some range restriction reasoning
-                assert forall i :: 0 <= i < |rule.body| ==> rule.body[i] == search_clauses[i].clause;
-                assert forall i :: 0 <= i < |rule.body| ==> valid_proof(rules, search_clauses[i].clause, proofs[i]);
-                assert forall i :: 0 <= i < |rule.body| ==> valid_proof(rules, rule.body[i], proofs[i]);
-                assert forall i :: 0 <= i < |rule.body| ==> rule.body[i].make_fact(concreteSubst) == Last(proofs[i]).new_fact();
+                // assert |proofs| == |search_clauses| == |rule.body|;
+                ////assert forall i :: 0 <= i < |rule.body| ==> rule.body[i] == search_clauses[i].clause;
+                // assert forall i :: 0 <= i < |rule.body| ==> search_clauses[i].valid_emap(emap);
+                // assume forall i :: 0 <= i < |rule.body| ==> search_clauses[i].emap_fully_resolved(emap); // TODO This will depend on some range restriction reasoning
+                //// assert forall i :: 0 <= i < |rule.body| ==> valid_proof(rules, search_clauses[i].clause.make_fact(make_subst(emap, search_clauses[i].subst)), proofs[i]);
+                //// assert forall i :: 0 <= i < |rule.body| ==> valid_proof(rules, search_clauses[i].clause.make_fact(concreteSubst), proofs[i]);
+                // assert forall i :: 0 <= i < |rule.body| ==> valid_proof(rules, rule.body[i], proofs[i]);
+                // assert forall i :: 0 <= i < |rule.body| ==> rule.body[i].make_fact(concreteSubst) == Last(proofs[i]).new_fact();
                 var proof := combine_proofs(rules, rule, concreteSubst, proofs);
+                assert(goal.subst.valid());
+                var goalSubst := make_subst(emap, goal.subst);
+                // assert();
+                // concreteSubst is concrete
+                // ==> forall vars in subst, subst[vars].Const?
+                // but subst[rule.head.terms[i]] == goal.subst[goal.clause.terms[i]] && |rule.head.terms| == |goal.clause.terms|
+                // and also |subst.Keys| == |goal.subst.Keys|
+                // therefore, all vars in goal.subst map to Consts
+                // assert forall e:VarTerm | subst.in1(e) :: emap.evar_map[subst.get1(e)].Some?;
+                // assert(forall e | e in goal.evar_terms :: e in subst.Values)
+                // assert goal.emap_fully_resolved(emap);
+                assert forall sc | sc in search_clauses :: forall v:VarTerm | v in sc.clause.terms :: concreteSubst[v].Const?;
+                // assert forall e | e in goal.subst.Values() :: (exists sc | sc in search_clauses :: e in sc.subst.Values());
+                // var pp:set<VarTerm>;
+                // for k := 0 to |search_clauses| 
+                //     invariant pp == 
+                // {
+                //     pp := pp + (ToSet(search_clauses[i].clause.terms));
+                // }
+                // assert(forall v:VarTerm | v in rule.head.terms :: (exists c | c in rule.body :: v in c.terms));
+                assert(seq(|search_clauses|, i requires 0 <= i < |search_clauses| => search_clauses[i].clause) == rule.body);
+                // assert(forall v:VarTerm | v in rule.head.terms :: match_exists(v, rule.body));
+                // assert(forall v:VarTerm | v in goal.clause.terms :: match_exists(v, seq(|search_clauses|, i => search_clauses[i].clause)));
+
+                // assert(forall v:VarTerm | v in rule.head.terms :: (exists c | c in rule.body :: v in c.terms));
+                // assert ToSet(goal.clause.terms) <= (set x:Term | ((forall sc :: sc in search_clauses && x in sc.clause.terms) :: x));
+                // set x : T | P(x) :: x
+                // assert forall t:VarTerm | t in goal.clause.terms :: emap.evar_map[goal.subst.get1(t)].Some?;
+                /* 
+                    assert forall i :: 0 <= i < |goal.clause.terms| ==> goal.subst.get1(goal.clause.terms[i]) == goal.evar_terms[i] == subst.get1(rule.head.terms[i])
+                    goal.clause.make_fact(goalSubst).terms[i] == emap.evar_map[goal.subst.get1(goal.clause.terms[i])]
+                    rule.head.make_fact(concreteSubst).terms[i] == emap.evar_map[subst.get1(rule.head.terms[i])]
+                    ==> goal.clause.make_fact(goalSubst).terms[i] == rule.head.make_fact(concreteSubst).terms[i]
+                */
+                assert goal.clause.substitution_concrete(goalSubst);
+                assert forall i :: 0 <= i < |goal.clause.terms| ==> goal.subst.get1(goal.clause.terms[i]) == goal.evar_terms[i] == subst.get1(rule.head.terms[i]);
+                assert forall i :: 0 <= i < |goal.clause.terms| ==> goal.clause.make_fact(goalSubst).terms[i] == Const(emap.evar_map[goal.subst.get1(goal.clause.terms[i])].value);
+                assert forall j :: 0 <= j < |rule.head.terms| ==> rule.head.terms[j].Const? ==> emap.evar_map[goal.evar_terms[j]].Some? && Const(emap.evar_map[goal.evar_terms[j]].value) == rule.head.terms[j];
+                assert forall i :: 0 <= i < |goal.clause.terms| ==> rule.head.make_fact(concreteSubst).terms[i] == Const(emap.evar_map[subst.get1(rule.head.terms[i])].value);
+                /*
+                    for all evars in goal.subst.Values, those evars also exist in search_clauses.subst.values for all search_clauses
+                 */
+
+                assert rule.head.make_fact(concreteSubst) == goal.clause.make_fact(goalSubst);
                 return true, Some(proof);
             }
         }
-        emap.copy(current_emap);
+        // emap.copy(current_emap);
     }
     return false, None;
 }
 
-ghost method flatten_two_proofs(rules: seq<Rule>, subst: Substitution, goal1: Clause, proof1: Proof, goal2: Clause, proof2: Proof) returns (proof: Proof)
+ghost method flatten_two_proofs(rules: seq<Rule>, subst: Substitution, goal1: Fact, proof1: Proof, goal2: Fact, proof2: Proof) returns (proof: Proof)
     requires valid_proof(rules, goal1, proof1)
     requires valid_proof(rules, goal2, proof2)
     requires goal1.substitution_concrete(subst)
@@ -317,24 +464,25 @@ ghost method flatten_two_proofs(rules: seq<Rule>, subst: Substitution, goal1: Cl
 ghost method combine_proofs(rules: seq<Rule>, rule: Rule, subst: Substitution, proofs: seq<Proof>) returns (proof: Proof)
     requires |rule.body| == |proofs| >= 1
     requires rule in rules
-    requires forall i :: 0 <= i < |rule.body| ==> valid_proof(rules, rule.body[i], proofs[i])
     requires rule.head.substitution_concrete(subst)
-    requires forall i :: 0 <= i < |rule.body| ==> rule.body[i].substitution_concrete(subst) && rule.body[i].make_fact(subst) == Last(proofs[i]).new_fact();
-    ensures  valid_proof(rules, rule.head, proof)
+    requires forall i :: 0 <= i < |rule.body| ==> rule.body[i].substitution_concrete(subst) 
+    requires forall i :: 0 <= i < |rule.body| ==> valid_proof(rules, rule.body[i].make_fact(subst), proofs[i])
+    requires forall i :: 0 <= i < |rule.body| ==> rule.body[i].make_fact(subst) == Last(proofs[i]).new_fact()
+    ensures  valid_proof(rules, rule.head.make_fact(subst), proof)
 {
     proof := proofs[0];
-    var goal := rule.body[0];
+    var goal := rule.body[0].make_fact(subst);
     for i := 1 to |proofs|
         invariant valid_proof(rules, goal, proof)
         invariant goal.substitution_concrete(subst)
         invariant goal.make_fact(subst) == Last(proof).new_fact()
-        invariant goal == rule.body[i-1]
+        invariant goal == rule.body[i-1].make_fact(subst)
         invariant forall j :: 0 <= j < |proof| ==> proof[j].valid()
         invariant forall j :: 0 <= j < i - 1 ==> rule.body[j].make_fact(subst) in Last(proof).facts
     {
-        var new_proof := flatten_two_proofs(rules, subst, rule.body[i], proofs[i], goal, proof);
+        var new_proof := flatten_two_proofs(rules, subst, rule.body[i].make_fact(subst), proofs[i], goal, proof);
         proof := new_proof;
-        goal := rule.body[i];
+        goal := rule.body[i].make_fact(subst);
     }
     var last_step := ProofStep(subst, rule, Last(proof).facts + [ Last(proof).new_fact() ]);
     proof := proof + [last_step];
@@ -342,28 +490,46 @@ ghost method combine_proofs(rules: seq<Rule>, rule: Rule, subst: Substitution, p
 
 method get_query_search_clause(query:Clause, emap:EvarMap) returns (sc:SearchClause)
     requires emap.inv()
+    requires valid_clause(query)
     modifies emap
     ensures emap.inv()
+    ensures sc.subst.valid()
+    ensures sc.valid()
     ensures sc.valid_emap(emap)
     ensures sc.clause == query
-    ensures sc.valid()
 {
+    reveal ToSet();
     var evar_terms:seq<Evar> := [];
-    var subst: EvarSubstitution := map[];
+    var subst: EvarSubstitution := new_bijective_map<VarTerm, Evar>();
+    assert(subst.Values() == {});
+    assert(ToSet(evar_terms) == {});
     for i := 0 to |query.terms|
         invariant emap.inv()
+        invariant subst.valid()
+        invariant |evar_terms| == i
+        invariant reveal ToSet(); ToSet(evar_terms) == subst.Values()
         invariant forall e:Evar :: e in evar_terms ==> e in emap.evar_map
-        invariant forall e:Evar :: e in subst.Values ==> e in emap.evar_map
-        invariant forall e:Evar :: e in subst.Values ==> e in evar_terms
+        invariant forall e:Evar :: subst.in2(e) ==> e in emap.evar_map
+        invariant forall e:Evar :: subst.in2(e) ==> e in evar_terms
+        invariant forall j :: i <= j < |query.terms| ==> !subst.in1(query.terms[j])
+        invariant forall j:nat | j < i :: (subst.in1(query.terms[j]) && subst.get1(query.terms[j]) == evar_terms[j])
+        invariant forall j:nat | j < i :: query.terms[j].Const? ==> emap.evar_map[evar_terms[j]] == Some(query.terms[j].c)
     {
         var term := query.terms[i];
         match term {
             case Var(s) => {
                         var new_ev := emap.get_new_evar();
                         evar_terms := evar_terms + [new_ev];
-                        subst := subst[term := new_ev];
+                        // subst := subst[term := new_ev];
+                        subst := subst.insert(term, new_ev);
                     }
-            case Const(c) => {} // TODO: Create new evars and map them to the const?
+            case Const(c) => {
+                        var new_ev := emap.get_new_evar();
+                        evar_terms := evar_terms + [new_ev];
+                        // subst := subst[term := new_ev];
+                        subst := subst.insert(term, new_ev);
+                        emap.resolve(new_ev, c);
+            } 
         }
     }
 
