dafny/top-down/top-down-old.dfy
@@ -1,0 +1,389 @@
+include "definitions.dfy"
+include "evar.dfy"
+include "search_clause.dfy"
+include "std-lib/src/Wrappers.dfy"
+include "std-lib/src/Collections/Sequences/Seq.dfy"
+import opened Wrappers
+import opened Seq
+
+/*
+
+Search procedure:
+
+global evar_map
+
+search(goal: SearchClause) returns (ghost proof: Option<ProofTree>, b: bool)
+  ensures b == True <==> (proof == Some(proof') && proof'.valid())
+{
+  // goal: R(arg1, arg2, ..., argN): where the args are evars in the evar_map
+  rules <- all rules with heads of the form R(arg1, arg2, ..., argN)
+  for rule in rules:
+    match unify(rule.Head, goal) with
+    | None => continue; // can't instantiate this rule due to conflicted ground terms
+    | Some(subst) =>
+      // subst is a map<var --> evar>
+      substitutedBody: seq<SearchClause> = evarify(rule.Body, subst);
+      for searchClause: SearchClause in substitutedBody:
+        search(searchClause)
+}
+
+*/
+
+method find_matching_rules(rules: seq<Rule>, goal:SearchClause) returns (c:seq<Rule>)
+    ensures forall r:Rule :: r in c ==> r.head.name == goal.name && |r.head.terms| == |goal.evar_terms|
+    ensures forall r:Rule :: r in c ==> r.head == goal.clause
+    ensures forall r:Rule :: r in c ==> r in rules
+{
+    var matching_rules : seq<Rule> := [];
+    
+    for i := 0 to |rules|
+        invariant forall r:Rule :: r in matching_rules ==> r.head.name == goal.name && |r.head.terms| == |goal.evar_terms|
+        invariant forall r:Rule :: r in matching_rules ==> r in rules
+    {
+        var rule := rules[i];
+        if (rule.head.name == goal.name && |rule.head.terms| == |goal.evar_terms|) {
+            matching_rules := matching_rules + [rule];
+        }
+    }
+    // TODO postcondition on goal.clause, based on bijective map stuff
+    return matching_rules;
+}
+
+
+method unify(head_clause:Clause, goal:SearchClause, emap:EvarMap) returns (o:Option<EvarSubstitution>)//, e:EvarMap)
+    requires emap.inv()
+    requires |head_clause.terms| == |goal.evar_terms|
+    requires goal.valid()
+    requires goal.valid_emap(emap)
+    modifies emap
+    ensures emap.is_more_resolved()
+    ensures goal.valid_emap(emap)
+    ensures emap.inv()
+    ensures o.Some? ==> forall e :: e in o.value.Values ==> e in emap.evar_map
+    ensures o.Some? ==> forall v :: v in goal.clause.terms && v.Var? ==> v in o.value
+    ensures head_clause.is_ground() && o.Some? ==> goal.emap_fully_resolved(emap)
+    ensures emap.monotonically_increasing() // ensures forall e :: e in old(emap.evar_map) ==> e in emap.evar_map
+{
+    // check if all terms in clause have correct mapping in goal.evar_terms
+    var subst:EvarSubstitution := map[];
+    for i := 0 to |head_clause.terms| 
+        invariant emap.inv()
+        invariant goal.valid_emap(emap)
+        invariant forall e :: e in subst.Values ==> e in emap.evar_map
+        invariant emap.monotonically_increasing() // invariant forall e :: e in old(emap.evar_map) ==> e in emap.evar_map
+        invariant emap.is_more_resolved()
+        invariant forall j :: 0 <= j < i ==> head_clause.terms[j].Const? ==> emap.evar_map[goal.evar_terms[j]].Some?
+    {
+        if head_clause.terms[i].Var? {
+            //print "a";
+            var variableName := head_clause.terms[i].s;
+            subst := subst[head_clause.terms[i] := goal.evar_terms[i]];
+        } else if head_clause.terms[i].Const? {
+            //print "b";
+            var constant := head_clause.terms[i].c;
+            var e := emap.lookup(goal.evar_terms[i]);
+            match e {
+                case None => {
+                    emap.resolve(goal.evar_terms[i], constant);
+                }
+                case Some(constant') =>
+                    if constant != constant' {
+                        // ignore rule
+                        return None;
+                    }
+                    // } else {
+                    //     subst := subst[head_clause.terms[i] := goal.evar_terms[i]];
+                    // }
+            }
+        }
+    }
+    reveal ToSet();
+    return Some(subst);
+}
+
+method evarify(clause:Clause, subst:EvarSubstitution, emap:EvarMap) 
+    returns (sc:SearchClause, subst':EvarSubstitution)
+    requires emap.inv()
+    requires forall e :: e in subst.Values ==> e in emap.evar_map
+    modifies emap
+    ensures  emap.inv()
+    ensures  sc.valid_emap(emap)
+    ensures  forall e :: e in subst'.Values ==> e in emap.evar_map
+    ensures  emap.monotonically_increasing() // ensures forall e :: e in old(emap.evar_map) ==> e in emap.evar_map
+    ensures  forall s :: s in subst ==> s in subst'
+    ensures  sc.clause == clause
+    ensures  sc.clause.substitution_complete(make_subst(emap, subst'))
+    ensures  sc.valid()
+{
+    subst' := subst;
+    var local_subst:EvarSubstitution := map[];
+    var evar_terms:seq<Evar> := [];
+    reveal ToSet();
+    for i := 0 to |clause.terms|
+        invariant emap.inv()
+        invariant forall e :: e in evar_terms ==> e in emap.evar_map
+        invariant forall e :: e in subst'.Values ==> e in emap.evar_map
+        invariant emap.monotonically_increasing() // invariant forall e :: e in old(emap.evar_map) ==> e in emap.evar_map 
+        invariant forall s :: s in subst ==> s in subst'
+        invariant forall j :: 0 <= j < i ==> clause.terms[j].Var? ==> clause.terms[j] in subst'
+        invariant forall e :: e in local_subst.Values ==> e in evar_terms
+    {
+        var term := clause.terms[i];
+        match term {
+            case Var(s) => {
+                if term in subst'.Keys {
+                    var ev := subst'[term]; // this should imply ev in emap.evar_map
+                    evar_terms := evar_terms + [ev];
+                    local_subst := local_subst[term := ev];
+                } else if term !in subst' {
+                    var new_ev := emap.get_new_evar();
+                    evar_terms := evar_terms + [new_ev];
+                    subst' := subst'[term := new_ev];
+                    local_subst := local_subst[term := new_ev];
+                }
+            }
+            case Const(c) => {
+                var new_ev := emap.get_new_evar();
+                evar_terms := evar_terms + [new_ev];
+                emap.resolve(new_ev, c);
+            }
+        }
+    }
+
+    sc := SearchClause(clause.name, evar_terms, clause, local_subst);
+}
+
+method search (rules:seq<Rule>, goal:SearchClause, emap:EvarMap, depth: nat) returns (b:bool, ghost proof: Option<Proof>)//, e:EvarMap)
+    requires valid_program(rules)
+    requires emap.inv()
+    requires goal.valid_emap(emap)
+    requires goal.valid()
+    // ensures o.Some? ==> forall e :: e in o.value.Values ==> e in emap.evar_map
+    modifies emap
+    ensures emap.inv()
+    ensures goal.valid_emap(emap) // TODO: Do we need to prove this at all times?
+    ensures emap.monotonically_increasing() // ensures forall e :: e in old(emap.evar_map) ==> e in emap.evar_map
+    ensures b ==> proof.Some? && valid_proof(rules, goal.clause, proof.value)
+    ensures b ==> goal.emap_fully_resolved(emap)
+    decreases depth
+    // what the correct matching rule is (rule for which we returned true)
+    //   - maybe return a sequence of these rules
+    //   - build a 'substitution' map like Bryan using these rules
+    //       - a substitution is either a variable->evar or evar->const(resolve)
+    //   - ??
+    //   - reuse Bryan's spec
+    // ensures b ==> that rule works
+
+    // the different subst bi-maps are consistent // WRONG
+    // we should somehow say b==true ==> at no point we made the same evar resolve to two diff consts
+    // for each subst (at each instantiation of a rule down the tree), convert that subst into Bryan's substitution (using the 'global' evarmap)
+    //  -- keep a ghost state of seq<subst * rule> or a seq<applied_rules> * seq<subst for that rule>?
+    //  -- (var -> evar -> const) ==> (var -> const) like Bryan's substitution (a ground substitution)
+    //  -- do the above for ALL evars in our evarmap, the one for which search returns true (basically for all evars we want them to be present in substs)
+    //  --   at each proofstep, the number of evars for which the above stuff is not done decreases
+    // prove completeness of our substs? - we get a valid ProofStep for free?
+{
+    if (depth == 0) {
+        return false, None;
+    }
+    //print "Searching on ", goal, " with emap ", emap.evar_map, "\n";
+    // find all rules that match current goal
+    var matching_rules := find_matching_rules(rules, goal);
+    //print "\t matching_rules = ", matching_rules, "\n";
+
+    // for all rules that match the current goal
+    for i := 0 to |matching_rules|
+        invariant emap.inv()
+        // invariant goal.valid_emap(emap)
+        invariant emap.monotonically_increasing() // invariant forall e :: e in old(emap.evar_map) ==> e in emap.evar_map
+    {
+        //print "\t i = ", i, "\n"; 
+        var current_emap:EvarMap := new EvarMap.Init(emap); // TODO: Check if this actually makes a copy
+        var rule:Rule := matching_rules[i];
+        //print "\t matching_rule = ", rule, "\n";
+        var option_subst := unify(rule.head, goal, emap);
+        
+        //print "\t option_subst = ", option_subst, "\n";
+        
+        var subst : EvarSubstitution;
+        match option_subst {
+            case None => continue;
+            case Some(subst') => subst := subst';
+        }
+
+        var search_clauses:seq<SearchClause> := [];
+        if |rule.body| == 0 {
+            var concreteSubst := make_subst(emap, subst);
+            var proofStep := ProofStep(concreteSubst, rule, []);
+            assert rule in rules; // needed to use valid_program(rules) to conclude that valid_rule(rule) and then conclude that rule.head.is_ground() 
+            return true, Some([proofStep]);
+        } else {
+            for j := 0 to |rule.body|
+                invariant |search_clauses| == j
+                invariant emap.inv()
+                invariant current_emap.inv()
+                // invariant current_emap.evar_map == old(current_emap.evar_map)
+                invariant forall sc :: sc in search_clauses ==> sc.valid_emap(emap)
+                invariant forall e :: e in subst.Values ==> e in emap.evar_map
+                invariant emap.monotonically_increasing() // invariant forall e :: e in old(emap.evar_map) ==> e in emap.evar_map
+                invariant forall e :: e in old(emap.evar_map) ==> e in current_emap.evar_map // TODO: Make this a predicate inside evar.dfy
+                invariant forall i :: 0 <= i < j ==> rule.body[i] == search_clauses[i].clause;
+                invariant forall i :: 0 <= i < j ==> search_clauses[i].clause.substitution_complete(make_subst(emap, subst))
+                invariant forall i :: 0 <= i < j ==> search_clauses[i].valid()
+            {
+                var clause:Clause := rule.body[j];
+                var search_clause, subst' := evarify(clause, subst, emap);
+                subst := subst';
+                search_clauses := search_clauses + [search_clause];
+            }
+            var flag := true;
+            ghost var proofs : seq<Proof> := [];
+            assert forall i :: 0 <= i < |search_clauses| ==> search_clauses[i].clause.substitution_complete(make_subst(emap, subst));
+            for j := 0 to |search_clauses|
+                invariant emap.inv()
+                invariant current_emap.inv()
+                // invariant current_emap == old(current_emap)
+                invariant forall sc :: sc in search_clauses ==> sc.valid_emap(emap)
+                // invariant forall e :: e in subst.Values ==> e in emap.evar_map
+                invariant emap.monotonically_increasing() // invariant forall e :: e in old(emap.evar_map) ==> e in emap.evar_map
+                invariant forall e :: e in old(emap.evar_map) ==> e in current_emap.evar_map // TODO: Make this a predicate inside evar.dfy
+                // invariant goal.valid_emap(emap)
+                invariant flag ==> (|proofs| == j)
+                invariant flag ==> (forall i :: 0 <= i < j ==> valid_proof(rules, search_clauses[i].clause, proofs[i]))
+                invariant flag ==> forall i :: 0 <= i < j ==> search_clauses[i].clause.make_fact(make_subst(emap, subst)) == Last(proofs[i]).new_fact();
+                invariant forall e :: e in subst.Values ==> e in emap.evar_map
+            {
+                var b',proof_j := search(rules, search_clauses[j], emap, depth - 1);
+                if !b' {
+                    flag := false;
+                    break;
+                } else {
+                    proofs := proofs + [proof_j.value];
+                }
+                // current_emap := e;
+            }
+            if flag {
+                var concreteSubst := make_subst(emap, subst);
+                assert |proofs| == |search_clauses| == |rule.body|;
+                assert forall i :: 0 <= i < |rule.body| ==> search_clauses[i].valid_emap(emap);
+                assume forall i :: 0 <= i < |rule.body| ==> search_clauses[i].emap_fully_resolved(emap); // TODO This will depend on some range restriction reasoning
+                assert forall i :: 0 <= i < |rule.body| ==> rule.body[i] == search_clauses[i].clause;
+                assert forall i :: 0 <= i < |rule.body| ==> valid_proof(rules, search_clauses[i].clause, proofs[i]);
+                assert forall i :: 0 <= i < |rule.body| ==> valid_proof(rules, rule.body[i], proofs[i]);
+                assert forall i :: 0 <= i < |rule.body| ==> rule.body[i].make_fact(concreteSubst) == Last(proofs[i]).new_fact();
+                var proof := combine_proofs(rules, rule, concreteSubst, proofs);
+                return true, Some(proof);
+            }
+        }
+        emap.copy(current_emap);
+    }
+    return false, None;
+}
+
+ghost method flatten_two_proofs(rules: seq<Rule>, subst: Substitution, goal1: Clause, proof1: Proof, goal2: Clause, proof2: Proof) returns (proof: Proof)
+    requires valid_proof(rules, goal1, proof1)
+    requires valid_proof(rules, goal2, proof2)
+    requires goal1.substitution_concrete(subst)
+    requires goal1.make_fact(subst) == Last(proof1).new_fact()
+    requires goal2.substitution_concrete(subst)
+    requires goal2.make_fact(subst) == Last(proof2).new_fact()
+    ensures  valid_proof(rules, goal1, proof)
+    ensures  goal1.make_fact(subst) == Last(proof).new_fact()
+    ensures  goal2.make_fact(subst) in Last(proof).facts
+    ensures  forall f :: f in Last(proof1).facts ==> f in Last(proof).facts
+    ensures  forall f :: f in Last(proof2).facts ==> f in Last(proof).facts
+{
+    var proof2_facts := Last(proof2).facts + [ Last(proof2).new_fact() ];
+    proof := proof2;
+    assert valid_proof(rules, goal2, proof);
+    assert forall j :: 0 <= j < |proof| ==> proof[j].rule in rules;
+    assert forall j :: 1 <= j < |proof| ==> proof[j].facts == proof[j-1].facts + [ proof[j-1].new_fact() ] ;
+    for i := 0 to |proof1|
+        invariant |proof| == |proof2| + i
+        invariant proof[..|proof2|] == proof2
+        invariant forall j :: 0 <= j < |proof| ==> proof[j].valid()
+        invariant forall j :: 0 <= j < |proof| ==> proof[j].rule in rules
+        invariant forall j :: 0 <= j < i ==> proof[|proof2| + j].facts == proof2_facts + proof1[j].facts
+        invariant forall j :: 0 <= j < i ==> proof1[j].new_fact() == proof[|proof2| + j].new_fact();
+        invariant forall j :: 1 <= j < |proof| ==> proof[j].facts == proof[j-1].facts + [ proof[j-1].new_fact() ] 
+        invariant forall j :: 0 <= j < i ==> proof[|proof2| + j].rule == proof1[j].rule
+    {
+        var proof_i_facts := proof2_facts + proof1[i].facts;
+        assert i > 0 ==> proof1[i].facts == proof1[i-1].facts + [ proof1[i-1].new_fact() ];        
+        proof := proof + [ProofStep(proof1[i].sub, proof1[i].rule, proof_i_facts)];
+    }
+}
+
+ghost method combine_proofs(rules: seq<Rule>, rule: Rule, subst: Substitution, proofs: seq<Proof>) returns (proof: Proof)
+    requires |rule.body| == |proofs| >= 1
+    requires rule in rules
+    requires forall i :: 0 <= i < |rule.body| ==> valid_proof(rules, rule.body[i], proofs[i])
+    requires rule.head.substitution_concrete(subst)
+    requires forall i :: 0 <= i < |rule.body| ==> rule.body[i].substitution_concrete(subst) && rule.body[i].make_fact(subst) == Last(proofs[i]).new_fact();
+    ensures  valid_proof(rules, rule.head, proof)
+{
+    proof := proofs[0];
+    var goal := rule.body[0];
+    for i := 1 to |proofs|
+        invariant valid_proof(rules, goal, proof)
+        invariant goal.substitution_concrete(subst)
+        invariant goal.make_fact(subst) == Last(proof).new_fact()
+        invariant goal == rule.body[i-1]
+        invariant forall j :: 0 <= j < |proof| ==> proof[j].valid()
+        invariant forall j :: 0 <= j < i - 1 ==> rule.body[j].make_fact(subst) in Last(proof).facts
+    {
+        var new_proof := flatten_two_proofs(rules, subst, rule.body[i], proofs[i], goal, proof);
+        proof := new_proof;
+        goal := rule.body[i];
+    }
+    var last_step := ProofStep(subst, rule, Last(proof).facts + [ Last(proof).new_fact() ]);
+    proof := proof + [last_step];
+}
+
+method get_query_search_clause(query:Clause, emap:EvarMap) returns (sc:SearchClause)
+    requires emap.inv()
+    modifies emap
+    ensures emap.inv()
+    ensures sc.valid_emap(emap)
+    ensures sc.clause == query
+    ensures sc.valid()
+{
+    var evar_terms:seq<Evar> := [];
+    var subst: EvarSubstitution := map[];
+    for i := 0 to |query.terms|
+        invariant emap.inv()
+        invariant forall e:Evar :: e in evar_terms ==> e in emap.evar_map
+        invariant forall e:Evar :: e in subst.Values ==> e in emap.evar_map
+        invariant forall e:Evar :: e in subst.Values ==> e in evar_terms
+    {
+        var term := query.terms[i];
+        match term {
+            case Var(s) => {
+                        var new_ev := emap.get_new_evar();
+                        evar_terms := evar_terms + [new_ev];
+                        subst := subst[term := new_ev];
+                    }
+            case Const(c) => {} // TODO: Create new evars and map them to the const?
+        }
+    }
+
+    reveal ToSet();
+    sc := SearchClause(query.name, evar_terms, query, subst);
+}
+
+method run_datalog(p:Program)
+    requires |p| > 0
+{
+    var prog := p;
+    var program_ok := check_program(prog);
+    if program_ok {
+        var query_rule := Last(p);
+        var emap:EvarMap := new EvarMap();
+        var query_sc:SearchClause := get_query_search_clause(query_rule.head, emap);
+        var b,proof := search(prog, query_sc, emap, 0x1_0000_0000);
+        assert (b == true ==> valid_query(prog, query_rule.head));
+        print "Query returned ", b, "\n";
+    } else {
+        print "Invalid or unsupported datalog program";
+    }
+}
